tests/AddDelay.bpl
@@ -11,7 +11,9 @@ var M: MType;
 var C: CType;
 var R: CType;
 var L: CType;
+var I: CType;
 var St: [Actor]State;
+
 const Base#L: int;
 axiom 1 <= Base#L;
 
@@ -26,7 +28,7 @@ function AT#Min(x:int, y: int): int { if x <= y then x else y }
 // ---------------------------------------------------------------
 
 procedure Add#anon$0#0()
-  modifies C, R, M, St;
+  modifies C, R, M, I, St;
 {
   var in1: Chan (int);
   var in2: Chan (int);
@@ -35,7 +37,7 @@ procedure Add#anon$0#0()
   assume true;
 }
 procedure Delay#anon$1#1()
-  modifies C, R, M, St;
+  modifies C, R, M, I, St;
 {
   var in: Chan (int);
   var out: Chan (int);
@@ -43,7 +45,7 @@ procedure Delay#anon$1#1()
   assume true;
 }
 procedure Delay#anon$2#2()
-  modifies C, R, M, St;
+  modifies C, R, M, I, St;
 {
   var in: Chan (int);
   var out: Chan (int);
@@ -51,9 +53,22 @@ procedure Delay#anon$2#2()
   assume true;
 }
 procedure Net#init#3()
-  modifies C, R, M, St;
+  modifies C, R, M, I, St;
 {
   var ActorParam#del#k: int;
+  assume 0 <= I[Net#a];
+  assume I[Net#a] <= R[Net#a];
+  assume R[Net#a] <= C[Net#a];
+  assume 0 <= I[Net#b];
+  assume I[Net#b] <= R[Net#b];
+  assume R[Net#b] <= C[Net#b];
+  assume 0 <= I[Net#c];
+  assume I[Net#c] <= R[Net#c];
+  assume R[Net#c] <= C[Net#c];
+  assume I[Net#c] == R[Net#c];
+  assume 0 <= I[Net#d];
+  assume I[Net#d] <= R[Net#d];
+  assume R[Net#d] <= C[Net#d];
   assume C[Net#a] == 0;
   assume R[Net#a] == 0;
   assume C[Net#b] == 0;
@@ -63,8 +78,27 @@ procedure Net#init#3()
   assume C[Net#d] == 0;
   assume R[Net#d] == 0;
   assume ActorParam#del#k == 0;
-  M[Net#b][R[Net#b] + C[Net#b]] := ActorParam#del#k;
+  M[Net#b][C[Net#b]] := ActorParam#del#k;
   C[Net#b] := C[Net#b] + 1;
+  assert {:msg "  Network initialization might not establish the channel invariant (#0)"} (forall i: int :: 
+    (0 <= i) && (i < C[Net#a]) ==> (0 < M[Net#a][i])
+  );
+  assert {:msg "  Network initialization might not establish the channel invariant (#1)"} R[Net#a] == C[Net#c];
+  assert {:msg "  Network initialization might not establish the channel invariant (#2)"} R[Net#b] == C[Net#c];
+  assert {:msg "  Network initialization might not establish the channel invariant (#3)"} R[Net#a] == C[Net#d];
+  assert {:msg "  Network initialization might not establish the channel invariant (#4)"} R[Net#b] == C[Net#d];
+  assert {:msg "  Network initialization might not establish the channel invariant (#5)"} R[Net#d] == (C[Net#b] - 1);
+  assert {:msg "  Network initialization might not establish the channel invariant (#6)"} (forall idx$: int :: 
+    (0 <= idx$) && (idx$ < C[Net#c]) ==> (M[Net#c][idx$] == (M[Net#a][idx$] + M[Net#b][idx$]))
+  );
+  assert {:msg "  Network initialization might not establish the channel invariant (#7)"} (forall idx$: int :: 
+    (0 <= idx$) && (idx$ < C[Net#d]) ==> (M[Net#d][idx$] == (M[Net#a][idx$] + M[Net#b][idx$]))
+  );
+  assert {:msg "  Network initialization might not establish the channel invariant (#8)"} (forall idx$: int :: 
+    (1 <= idx$) && (idx$ < C[Net#b]) ==> (M[Net#b][idx$] == M[Net#d][idx$ - 1])
+  );
+  assert {:msg "  22.15: Network initialization might not establish the channel invariant (#9)"} I[Net#a] == I[Net#c];
+  assert {:msg "  23.15: Network initialization might not establish the channel invariant (#10)"} M[Net#b][0] == 0;
   C[Net#b] := C[Net#b] - 1;
 }
 const unique Net#add: Actor;
@@ -74,245 +108,276 @@ const unique Net#b: Chan (int);
 const unique Net#c: Chan (int);
 const unique Net#d: Chan (int);
 procedure Net#anon$3#entry#4()
-  modifies C, R, M, St;
+  modifies C, R, M, I, St;
 {
+  assume 0 <= I[Net#a];
+  assume I[Net#a] <= R[Net#a];
+  assume R[Net#a] <= C[Net#a];
+  assume 0 <= I[Net#b];
+  assume I[Net#b] <= R[Net#b];
+  assume R[Net#b] <= C[Net#b];
+  assume 0 <= I[Net#c];
+  assume I[Net#c] <= R[Net#c];
+  assume R[Net#c] <= C[Net#c];
+  assume I[Net#c] == R[Net#c];
+  assume 0 <= I[Net#d];
+  assume I[Net#d] <= R[Net#d];
+  assume R[Net#d] <= C[Net#d];
   assume L[Net#a] == (1 * Base#L);
-  assume C[Net#a] == 0;
-  assume C[Net#b] == 0;
-  assume C[Net#c] == 0;
-  assume C[Net#d] == 0;
+  assume (R[Net#a] - I[Net#a]) <= L[Net#a];
+  assume (C[Net#a] - R[Net#a]) == 0;
+  assume (C[Net#b] - R[Net#b]) == 0;
+  assume (C[Net#c] - R[Net#c]) == 0;
+  assume (C[Net#d] - R[Net#d]) == 0;
+  assume I == R;
   C[Net#b] := C[Net#b] + 1;
-  assume 0 <= R[Net#a];
-  assume 0 <= C[Net#a];
-  assume (R[Net#a] + C[Net#a]) <= L[Net#a];
-  assume 0 <= R[Net#b];
-  assume 0 <= C[Net#b];
-  assume 0 <= R[Net#c];
-  assume 0 <= C[Net#c];
-  assume R[Net#c] == 0;
-  assume 0 <= R[Net#d];
-  assume 0 <= C[Net#d];
   assume (forall i: int :: 
-    (0 <= i) && (i < L[Net#a]) ==> (0 < M[Net#a][i])
+    (0 <= i) && (i < C[Net#a]) ==> (0 < M[Net#a][i])
   );
-  assume R[Net#a] == (R[Net#c] + C[Net#c]);
-  assume R[Net#b] == (R[Net#c] + C[Net#c]);
-  assume R[Net#a] == (R[Net#d] + C[Net#d]);
-  assume R[Net#b] == (R[Net#d] + C[Net#d]);
-  assume R[Net#d] == ((R[Net#b] + C[Net#b]) - 1);
+  assume R[Net#a] == C[Net#c];
+  assume R[Net#b] == C[Net#c];
+  assume R[Net#a] == C[Net#d];
+  assume R[Net#b] == C[Net#d];
+  assume R[Net#d] == (C[Net#b] - 1);
   assume (forall idx$: int :: 
-    (0 <= idx$) && (idx$ < (R[Net#c] + C[Net#c])) ==> (M[Net#c][idx$] == (M[Net#a][idx$] + M[Net#b][idx$]))
-  );
-  assume (forall idx$: int :: 
-    (0 <= idx$) && (idx$ < (R[Net#d] + C[Net#d])) ==> (M[Net#d][idx$] == (M[Net#a][idx$] + M[Net#b][idx$]))
+    (0 <= idx$) && (idx$ < C[Net#c]) ==> (M[Net#c][idx$] == (M[Net#a][idx$] + M[Net#b][idx$]))
   );
   assume (forall idx$: int :: 
-    (1 <= idx$) && (idx$ < (R[Net#b] + C[Net#b])) ==> (M[Net#b][idx$] == M[Net#d][idx$ - 1])
+    (0 <= idx$) && (idx$ < C[Net#d]) ==> (M[Net#d][idx$] == (M[Net#a][idx$] + M[Net#b][idx$]))
   );
+  assume (forall idx$: int :: 
+    (1 <= idx$) && (idx$ < C[Net#b]) ==> (M[Net#b][idx$] == M[Net#d][idx$ - 1])
+  );
+  assume I[Net#a] == I[Net#c];
+  assume M[Net#b][0] == 0;
   assume (forall i: int :: 
-    (0 <= i) && (i < L[Net#a]) ==> (0 < M[Net#a][i])
+    (0 <= i) && (i < C[Net#a]) ==> (0 < M[Net#a][i])
   );
-  assert {:msg "  Channel invariant might not hold on action entry (#0)"} (forall i: int :: 
-    (0 <= i) && (i < L[Net#a]) ==> (0 < M[Net#a][i])
+  assert {:msg "  Channel invariant might not hold on action entry (#11)"} (forall i: int :: 
+    (0 <= i) && (i < C[Net#a]) ==> (0 < M[Net#a][i])
   );
-  assert {:msg "  Channel invariant might not hold on action entry (#1)"} R[Net#a] == (R[Net#c] + C[Net#c]);
-  assert {:msg "  Channel invariant might not hold on action entry (#2)"} R[Net#b] == (R[Net#c] + C[Net#c]);
-  assert {:msg "  Channel invariant might not hold on action entry (#3)"} R[Net#a] == (R[Net#d] + C[Net#d]);
-  assert {:msg "  Channel invariant might not hold on action entry (#4)"} R[Net#b] == (R[Net#d] + C[Net#d]);
-  assert {:msg "  Channel invariant might not hold on action entry (#5)"} R[Net#d] == ((R[Net#b] + C[Net#b]) - 1);
-  assert {:msg "  Channel invariant might not hold on action entry (#6)"} (forall idx$: int :: 
-    (0 <= idx$) && (idx$ < (R[Net#c] + C[Net#c])) ==> (M[Net#c][idx$] == (M[Net#a][idx$] + M[Net#b][idx$]))
+  assert {:msg "  Channel invariant might not hold on action entry (#12)"} R[Net#a] == C[Net#c];
+  assert {:msg "  Channel invariant might not hold on action entry (#13)"} R[Net#b] == C[Net#c];
+  assert {:msg "  Channel invariant might not hold on action entry (#14)"} R[Net#a] == C[Net#d];
+  assert {:msg "  Channel invariant might not hold on action entry (#15)"} R[Net#b] == C[Net#d];
+  assert {:msg "  Channel invariant might not hold on action entry (#16)"} R[Net#d] == (C[Net#b] - 1);
+  assert {:msg "  Channel invariant might not hold on action entry (#17)"} (forall idx$: int :: 
+    (0 <= idx$) && (idx$ < C[Net#c]) ==> (M[Net#c][idx$] == (M[Net#a][idx$] + M[Net#b][idx$]))
   );
-  assert {:msg "  Channel invariant might not hold on action entry (#7)"} (forall idx$: int :: 
-    (0 <= idx$) && (idx$ < (R[Net#d] + C[Net#d])) ==> (M[Net#d][idx$] == (M[Net#a][idx$] + M[Net#b][idx$]))
+  assert {:msg "  Channel invariant might not hold on action entry (#18)"} (forall idx$: int :: 
+    (0 <= idx$) && (idx$ < C[Net#d]) ==> (M[Net#d][idx$] == (M[Net#a][idx$] + M[Net#b][idx$]))
   );
-  assert {:msg "  Channel invariant might not hold on action entry (#8)"} (forall idx$: int :: 
-    (1 <= idx$) && (idx$ < (R[Net#b] + C[Net#b])) ==> (M[Net#b][idx$] == M[Net#d][idx$ - 1])
+  assert {:msg "  Channel invariant might not hold on action entry (#19)"} (forall idx$: int :: 
+    (1 <= idx$) && (idx$ < C[Net#b]) ==> (M[Net#b][idx$] == M[Net#d][idx$ - 1])
   );
+  assert {:msg "  22.15: Channel invariant might not hold on action entry (#20)"} I[Net#a] == I[Net#c];
+  assert {:msg "  23.15: Channel invariant might not hold on action entry (#21)"} M[Net#b][0] == 0;
 }
 procedure Net#anon$3#Add#anon$0#5()
-  modifies C, R, M, St;
+  modifies C, R, M, I, St;
 {
   var St#next: State;
   var in1#i: int;
   var in2#j: int;
+  assume 0 <= I[Net#a];
+  assume I[Net#a] <= R[Net#a];
+  assume R[Net#a] <= C[Net#a];
+  assume 0 <= I[Net#b];
+  assume I[Net#b] <= R[Net#b];
+  assume R[Net#b] <= C[Net#b];
+  assume 0 <= I[Net#c];
+  assume I[Net#c] <= R[Net#c];
+  assume R[Net#c] <= C[Net#c];
+  assume I[Net#c] == R[Net#c];
+  assume 0 <= I[Net#d];
+  assume I[Net#d] <= R[Net#d];
+  assume R[Net#d] <= C[Net#d];
   assume L[Net#a] == (1 * Base#L);
-  assume 0 <= R[Net#a];
-  assume 0 <= C[Net#a];
-  assume (R[Net#a] + C[Net#a]) <= L[Net#a];
-  assume 0 <= R[Net#b];
-  assume 0 <= C[Net#b];
-  assume 0 <= R[Net#c];
-  assume 0 <= C[Net#c];
-  assume R[Net#c] == 0;
-  assume 0 <= R[Net#d];
-  assume 0 <= C[Net#d];
+  assume (R[Net#a] - I[Net#a]) <= L[Net#a];
   assume (forall i: int :: 
-    (0 <= i) && (i < L[Net#a]) ==> (0 < M[Net#a][i])
+    (0 <= i) && (i < C[Net#a]) ==> (0 < M[Net#a][i])
   );
-  assume R[Net#a] == (R[Net#c] + C[Net#c]);
-  assume R[Net#b] == (R[Net#c] + C[Net#c]);
-  assume R[Net#a] == (R[Net#d] + C[Net#d]);
-  assume R[Net#b] == (R[Net#d] + C[Net#d]);
-  assume R[Net#d] == ((R[Net#b] + C[Net#b]) - 1);
+  assume R[Net#a] == C[Net#c];
+  assume R[Net#b] == C[Net#c];
+  assume R[Net#a] == C[Net#d];
+  assume R[Net#b] == C[Net#d];
+  assume R[Net#d] == (C[Net#b] - 1);
   assume (forall idx$: int :: 
-    (0 <= idx$) && (idx$ < (R[Net#c] + C[Net#c])) ==> (M[Net#c][idx$] == (M[Net#a][idx$] + M[Net#b][idx$]))
-  );
-  assume (forall idx$: int :: 
-    (0 <= idx$) && (idx$ < (R[Net#d] + C[Net#d])) ==> (M[Net#d][idx$] == (M[Net#a][idx$] + M[Net#b][idx$]))
+    (0 <= idx$) && (idx$ < C[Net#c]) ==> (M[Net#c][idx$] == (M[Net#a][idx$] + M[Net#b][idx$]))
   );
   assume (forall idx$: int :: 
-    (1 <= idx$) && (idx$ < (R[Net#b] + C[Net#b])) ==> (M[Net#b][idx$] == M[Net#d][idx$ - 1])
+    (0 <= idx$) && (idx$ < C[Net#d]) ==> (M[Net#d][idx$] == (M[Net#a][idx$] + M[Net#b][idx$]))
   );
+  assume (forall idx$: int :: 
+    (1 <= idx$) && (idx$ < C[Net#b]) ==> (M[Net#b][idx$] == M[Net#d][idx$ - 1])
+  );
+  assume I[Net#a] == I[Net#c];
+  assume M[Net#b][0] == 0;
   assume true;
-  assume (1 <= C[Net#a]) && (1 <= C[Net#b]);
+  assume (1 <= (C[Net#a] - R[Net#a])) && (1 <= (C[Net#b] - R[Net#b]));
   in1#i := M[Net#a][R[Net#a]];
   R[Net#a] := R[Net#a] + 1;
-  C[Net#a] := C[Net#a] - 1;
   in2#j := M[Net#b][R[Net#b]];
   R[Net#b] := R[Net#b] + 1;
-  C[Net#b] := C[Net#b] - 1;
-  M[Net#c][R[Net#c] + C[Net#c]] := in1#i + in2#j;
+  M[Net#c][C[Net#c]] := in1#i + in2#j;
   C[Net#c] := C[Net#c] + 1;
-  M[Net#d][R[Net#d] + C[Net#d]] := in1#i + in2#j;
+  M[Net#d][C[Net#d]] := in1#i + in2#j;
   C[Net#d] := C[Net#d] + 1;
-  assert {:msg "  Action at 3.3 ('anon$0') for actor instance 'add' might not preserve the channel invariant (#9)"} (forall i: int :: 
-    (0 <= i) && (i < L[Net#a]) ==> (0 < M[Net#a][i])
+  assert {:msg "  Action at 3.3 ('anon$0') for actor instance 'add' might not preserve the channel invariant (#22)"} (forall i: int :: 
+    (0 <= i) && (i < C[Net#a]) ==> (0 < M[Net#a][i])
   );
-  assert {:msg "  Action at 3.3 ('anon$0') for actor instance 'add' might not preserve the channel invariant (#10)"} R[Net#a] == (R[Net#c] + C[Net#c]);
-  assert {:msg "  Action at 3.3 ('anon$0') for actor instance 'add' might not preserve the channel invariant (#11)"} R[Net#b] == (R[Net#c] + C[Net#c]);
-  assert {:msg "  Action at 3.3 ('anon$0') for actor instance 'add' might not preserve the channel invariant (#12)"} R[Net#a] == (R[Net#d] + C[Net#d]);
-  assert {:msg "  Action at 3.3 ('anon$0') for actor instance 'add' might not preserve the channel invariant (#13)"} R[Net#b] == (R[Net#d] + C[Net#d]);
-  assert {:msg "  Action at 3.3 ('anon$0') for actor instance 'add' might not preserve the channel invariant (#14)"} R[Net#d] == ((R[Net#b] + C[Net#b]) - 1);
-  assert {:msg "  Action at 3.3 ('anon$0') for actor instance 'add' might not preserve the channel invariant (#15)"} (forall idx$: int :: 
-    (0 <= idx$) && (idx$ < (R[Net#c] + C[Net#c])) ==> (M[Net#c][idx$] == (M[Net#a][idx$] + M[Net#b][idx$]))
+  assert {:msg "  Action at 3.3 ('anon$0') for actor instance 'add' might not preserve the channel invariant (#23)"} R[Net#a] == C[Net#c];
+  assert {:msg "  Action at 3.3 ('anon$0') for actor instance 'add' might not preserve the channel invariant (#24)"} R[Net#b] == C[Net#c];
+  assert {:msg "  Action at 3.3 ('anon$0') for actor instance 'add' might not preserve the channel invariant (#25)"} R[Net#a] == C[Net#d];
+  assert {:msg "  Action at 3.3 ('anon$0') for actor instance 'add' might not preserve the channel invariant (#26)"} R[Net#b] == C[Net#d];
+  assert {:msg "  Action at 3.3 ('anon$0') for actor instance 'add' might not preserve the channel invariant (#27)"} R[Net#d] == (C[Net#b] - 1);
+  assert {:msg "  Action at 3.3 ('anon$0') for actor instance 'add' might not preserve the channel invariant (#28)"} (forall idx$: int :: 
+    (0 <= idx$) && (idx$ < C[Net#c]) ==> (M[Net#c][idx$] == (M[Net#a][idx$] + M[Net#b][idx$]))
   );
-  assert {:msg "  Action at 3.3 ('anon$0') for actor instance 'add' might not preserve the channel invariant (#16)"} (forall idx$: int :: 
-    (0 <= idx$) && (idx$ < (R[Net#d] + C[Net#d])) ==> (M[Net#d][idx$] == (M[Net#a][idx$] + M[Net#b][idx$]))
+  assert {:msg "  Action at 3.3 ('anon$0') for actor instance 'add' might not preserve the channel invariant (#29)"} (forall idx$: int :: 
+    (0 <= idx$) && (idx$ < C[Net#d]) ==> (M[Net#d][idx$] == (M[Net#a][idx$] + M[Net#b][idx$]))
   );
-  assert {:msg "  Action at 3.3 ('anon$0') for actor instance 'add' might not preserve the channel invariant (#17)"} (forall idx$: int :: 
-    (1 <= idx$) && (idx$ < (R[Net#b] + C[Net#b])) ==> (M[Net#b][idx$] == M[Net#d][idx$ - 1])
+  assert {:msg "  Action at 3.3 ('anon$0') for actor instance 'add' might not preserve the channel invariant (#30)"} (forall idx$: int :: 
+    (1 <= idx$) && (idx$ < C[Net#b]) ==> (M[Net#b][idx$] == M[Net#d][idx$ - 1])
   );
+  assert {:msg "  22.15: Action at 3.3 ('anon$0') for actor instance 'add' might not preserve the channel invariant (#31)"} I[Net#a] == I[Net#c];
+  assert {:msg "  23.15: Action at 3.3 ('anon$0') for actor instance 'add' might not preserve the channel invariant (#32)"} M[Net#b][0] == 0;
 }
 procedure Net#anon$3#Delay#anon$2#6()
-  modifies C, R, M, St;
+  modifies C, R, M, I, St;
 {
   var ActorParam#k: int;
   var St#next: State;
   var in#i: int;
+  assume 0 <= I[Net#a];
+  assume I[Net#a] <= R[Net#a];
+  assume R[Net#a] <= C[Net#a];
+  assume 0 <= I[Net#b];
+  assume I[Net#b] <= R[Net#b];
+  assume R[Net#b] <= C[Net#b];
+  assume 0 <= I[Net#c];
+  assume I[Net#c] <= R[Net#c];
+  assume R[Net#c] <= C[Net#c];
+  assume I[Net#c] == R[Net#c];
+  assume 0 <= I[Net#d];
+  assume I[Net#d] <= R[Net#d];
+  assume R[Net#d] <= C[Net#d];
   assume ActorParam#k == 0;
   assume L[Net#a] == (1 * Base#L);
-  assume 0 <= R[Net#a];
-  assume 0 <= C[Net#a];
-  assume (R[Net#a] + C[Net#a]) <= L[Net#a];
-  assume 0 <= R[Net#b];
-  assume 0 <= C[Net#b];
-  assume 0 <= R[Net#c];
-  assume 0 <= C[Net#c];
-  assume R[Net#c] == 0;
-  assume 0 <= R[Net#d];
-  assume 0 <= C[Net#d];
+  assume (R[Net#a] - I[Net#a]) <= L[Net#a];
   assume (forall i: int :: 
-    (0 <= i) && (i < L[Net#a]) ==> (0 < M[Net#a][i])
+    (0 <= i) && (i < C[Net#a]) ==> (0 < M[Net#a][i])
   );
-  assume R[Net#a] == (R[Net#c] + C[Net#c]);
-  assume R[Net#b] == (R[Net#c] + C[Net#c]);
-  assume R[Net#a] == (R[Net#d] + C[Net#d]);
-  assume R[Net#b] == (R[Net#d] + C[Net#d]);
-  assume R[Net#d] == ((R[Net#b] + C[Net#b]) - 1);
+  assume R[Net#a] == C[Net#c];
+  assume R[Net#b] == C[Net#c];
+  assume R[Net#a] == C[Net#d];
+  assume R[Net#b] == C[Net#d];
+  assume R[Net#d] == (C[Net#b] - 1);
   assume (forall idx$: int :: 
-    (0 <= idx$) && (idx$ < (R[Net#c] + C[Net#c])) ==> (M[Net#c][idx$] == (M[Net#a][idx$] + M[Net#b][idx$]))
-  );
-  assume (forall idx$: int :: 
-    (0 <= idx$) && (idx$ < (R[Net#d] + C[Net#d])) ==> (M[Net#d][idx$] == (M[Net#a][idx$] + M[Net#b][idx$]))
+    (0 <= idx$) && (idx$ < C[Net#c]) ==> (M[Net#c][idx$] == (M[Net#a][idx$] + M[Net#b][idx$]))
   );
   assume (forall idx$: int :: 
-    (1 <= idx$) && (idx$ < (R[Net#b] + C[Net#b])) ==> (M[Net#b][idx$] == M[Net#d][idx$ - 1])
+    (0 <= idx$) && (idx$ < C[Net#d]) ==> (M[Net#d][idx$] == (M[Net#a][idx$] + M[Net#b][idx$]))
   );
+  assume (forall idx$: int :: 
+    (1 <= idx$) && (idx$ < C[Net#b]) ==> (M[Net#b][idx$] == M[Net#d][idx$ - 1])
+  );
+  assume I[Net#a] == I[Net#c];
+  assume M[Net#b][0] == 0;
   assume true;
-  assume 1 <= C[Net#d];
+  assume 1 <= (C[Net#d] - R[Net#d]);
   in#i := M[Net#d][R[Net#d]];
   R[Net#d] := R[Net#d] + 1;
-  C[Net#d] := C[Net#d] - 1;
-  M[Net#b][R[Net#b] + C[Net#b]] := in#i;
+  M[Net#b][C[Net#b]] := in#i;
   C[Net#b] := C[Net#b] + 1;
-  assert {:msg "  Action at 9.3 ('anon$2') for actor instance 'del' might not preserve the channel invariant (#18)"} (forall i: int :: 
-    (0 <= i) && (i < L[Net#a]) ==> (0 < M[Net#a][i])
+  assert {:msg "  Action at 9.3 ('anon$2') for actor instance 'del' might not preserve the channel invariant (#33)"} (forall i: int :: 
+    (0 <= i) && (i < C[Net#a]) ==> (0 < M[Net#a][i])
   );
-  assert {:msg "  Action at 9.3 ('anon$2') for actor instance 'del' might not preserve the channel invariant (#19)"} R[Net#a] == (R[Net#c] + C[Net#c]);
-  assert {:msg "  Action at 9.3 ('anon$2') for actor instance 'del' might not preserve the channel invariant (#20)"} R[Net#b] == (R[Net#c] + C[Net#c]);
-  assert {:msg "  Action at 9.3 ('anon$2') for actor instance 'del' might not preserve the channel invariant (#21)"} R[Net#a] == (R[Net#d] + C[Net#d]);
-  assert {:msg "  Action at 9.3 ('anon$2') for actor instance 'del' might not preserve the channel invariant (#22)"} R[Net#b] == (R[Net#d] + C[Net#d]);
-  assert {:msg "  Action at 9.3 ('anon$2') for actor instance 'del' might not preserve the channel invariant (#23)"} R[Net#d] == ((R[Net#b] + C[Net#b]) - 1);
-  assert {:msg "  Action at 9.3 ('anon$2') for actor instance 'del' might not preserve the channel invariant (#24)"} (forall idx$: int :: 
-    (0 <= idx$) && (idx$ < (R[Net#c] + C[Net#c])) ==> (M[Net#c][idx$] == (M[Net#a][idx$] + M[Net#b][idx$]))
+  assert {:msg "  Action at 9.3 ('anon$2') for actor instance 'del' might not preserve the channel invariant (#34)"} R[Net#a] == C[Net#c];
+  assert {:msg "  Action at 9.3 ('anon$2') for actor instance 'del' might not preserve the channel invariant (#35)"} R[Net#b] == C[Net#c];
+  assert {:msg "  Action at 9.3 ('anon$2') for actor instance 'del' might not preserve the channel invariant (#36)"} R[Net#a] == C[Net#d];
+  assert {:msg "  Action at 9.3 ('anon$2') for actor instance 'del' might not preserve the channel invariant (#37)"} R[Net#b] == C[Net#d];
+  assert {:msg "  Action at 9.3 ('anon$2') for actor instance 'del' might not preserve the channel invariant (#38)"} R[Net#d] == (C[Net#b] - 1);
+  assert {:msg "  Action at 9.3 ('anon$2') for actor instance 'del' might not preserve the channel invariant (#39)"} (forall idx$: int :: 
+    (0 <= idx$) && (idx$ < C[Net#c]) ==> (M[Net#c][idx$] == (M[Net#a][idx$] + M[Net#b][idx$]))
   );
-  assert {:msg "  Action at 9.3 ('anon$2') for actor instance 'del' might not preserve the channel invariant (#25)"} (forall idx$: int :: 
-    (0 <= idx$) && (idx$ < (R[Net#d] + C[Net#d])) ==> (M[Net#d][idx$] == (M[Net#a][idx$] + M[Net#b][idx$]))
+  assert {:msg "  Action at 9.3 ('anon$2') for actor instance 'del' might not preserve the channel invariant (#40)"} (forall idx$: int :: 
+    (0 <= idx$) && (idx$ < C[Net#d]) ==> (M[Net#d][idx$] == (M[Net#a][idx$] + M[Net#b][idx$]))
   );
-  assert {:msg "  Action at 9.3 ('anon$2') for actor instance 'del' might not preserve the channel invariant (#26)"} (forall idx$: int :: 
-    (1 <= idx$) && (idx$ < (R[Net#b] + C[Net#b])) ==> (M[Net#b][idx$] == M[Net#d][idx$ - 1])
+  assert {:msg "  Action at 9.3 ('anon$2') for actor instance 'del' might not preserve the channel invariant (#41)"} (forall idx$: int :: 
+    (1 <= idx$) && (idx$ < C[Net#b]) ==> (M[Net#b][idx$] == M[Net#d][idx$ - 1])
   );
+  assert {:msg "  22.15: Action at 9.3 ('anon$2') for actor instance 'del' might not preserve the channel invariant (#42)"} I[Net#a] == I[Net#c];
+  assert {:msg "  23.15: Action at 9.3 ('anon$2') for actor instance 'del' might not preserve the channel invariant (#43)"} M[Net#b][0] == 0;
 }
 procedure Net#anon$3#exit#7()
-  modifies C, R, M, St;
+  modifies C, R, M, I, St;
 {
+  assume 0 <= I[Net#a];
+  assume I[Net#a] <= R[Net#a];
+  assume R[Net#a] <= C[Net#a];
+  assume 0 <= I[Net#b];
+  assume I[Net#b] <= R[Net#b];
+  assume R[Net#b] <= C[Net#b];
+  assume 0 <= I[Net#c];
+  assume I[Net#c] <= R[Net#c];
+  assume R[Net#c] <= C[Net#c];
+  assume I[Net#c] == R[Net#c];
+  assume 0 <= I[Net#d];
+  assume I[Net#d] <= R[Net#d];
+  assume R[Net#d] <= C[Net#d];
   assume L[Net#a] == (1 * Base#L);
-  assume 0 <= R[Net#a];
-  assume 0 <= C[Net#a];
-  assume (R[Net#a] + C[Net#a]) <= L[Net#a];
-  assume 0 <= R[Net#b];
-  assume 0 <= C[Net#b];
-  assume 0 <= R[Net#c];
-  assume 0 <= C[Net#c];
-  assume R[Net#c] == 0;
-  assume 0 <= R[Net#d];
-  assume 0 <= C[Net#d];
+  assume (R[Net#a] - I[Net#a]) <= L[Net#a];
   assume (forall i: int :: 
-    (0 <= i) && (i < L[Net#a]) ==> (0 < M[Net#a][i])
+    (0 <= i) && (i < C[Net#a]) ==> (0 < M[Net#a][i])
   );
-  assume R[Net#a] == (R[Net#c] + C[Net#c]);
-  assume R[Net#b] == (R[Net#c] + C[Net#c]);
-  assume R[Net#a] == (R[Net#d] + C[Net#d]);
-  assume R[Net#b] == (R[Net#d] + C[Net#d]);
-  assume R[Net#d] == ((R[Net#b] + C[Net#b]) - 1);
+  assume R[Net#a] == C[Net#c];
+  assume R[Net#b] == C[Net#c];
+  assume R[Net#a] == C[Net#d];
+  assume R[Net#b] == C[Net#d];
+  assume R[Net#d] == (C[Net#b] - 1);
   assume (forall idx$: int :: 
-    (0 <= idx$) && (idx$ < (R[Net#c] + C[Net#c])) ==> (M[Net#c][idx$] == (M[Net#a][idx$] + M[Net#b][idx$]))
-  );
-  assume (forall idx$: int :: 
-    (0 <= idx$) && (idx$ < (R[Net#d] + C[Net#d])) ==> (M[Net#d][idx$] == (M[Net#a][idx$] + M[Net#b][idx$]))
+    (0 <= idx$) && (idx$ < C[Net#c]) ==> (M[Net#c][idx$] == (M[Net#a][idx$] + M[Net#b][idx$]))
   );
   assume (forall idx$: int :: 
-    (1 <= idx$) && (idx$ < (R[Net#b] + C[Net#b])) ==> (M[Net#b][idx$] == M[Net#d][idx$ - 1])
+    (0 <= idx$) && (idx$ < C[Net#d]) ==> (M[Net#d][idx$] == (M[Net#a][idx$] + M[Net#b][idx$]))
   );
-  assume !((R[Net#a] + C[Net#a]) < L[Net#a]);
-  assume !((1 <= C[Net#a]) && (1 <= C[Net#b]));
-  assume !(1 <= C[Net#d]);
-  assert {:msg "  21.14: Network action postcondition might not hold"} (forall i: int :: 
-    (1 <= i) && (i < (R[Net#c] + C[Net#c])) ==> (M[Net#c][i] == (M[Net#a][i] + M[Net#c][i - 1]))
+  assume (forall idx$: int :: 
+    (1 <= idx$) && (idx$ < C[Net#b]) ==> (M[Net#b][idx$] == M[Net#d][idx$ - 1])
   );
-  R[Net#c] := R[Net#c] + C[Net#c];
-  C[Net#c] := C[Net#c] - (1 * Base#L);
-  assert {:msg "  The network might not preserve the channel invariant"} (forall i: int :: 
-    (0 <= i) && (i < L[Net#a]) ==> (0 < M[Net#a][i])
+  assume I[Net#a] == I[Net#c];
+  assume M[Net#b][0] == 0;
+  assume !((R[Net#a] - I[Net#a]) < L[Net#a]);
+  assume !((1 <= (C[Net#a] - R[Net#a])) && (1 <= (C[Net#b] - R[Net#b])));
+  assume !(1 <= (C[Net#d] - R[Net#d]));
+  assert {:msg "  16.13: Network action postcondition might not hold"} M[Net#c][0] == M[Net#a][0];
+  assert {:msg "  17.14: Network action postcondition might not hold"} (forall i: int :: 
+    (1 <= i) && (i < C[Net#c]) ==> (M[Net#c][i] == (M[Net#a][i] + M[Net#c][i - 1]))
   );
-  assert {:msg "  The network might not preserve the channel invariant"} R[Net#a] == (R[Net#c] + C[Net#c]);
-  assert {:msg "  The network might not preserve the channel invariant"} R[Net#b] == (R[Net#c] + C[Net#c]);
-  assert {:msg "  The network might not preserve the channel invariant"} R[Net#a] == (R[Net#d] + C[Net#d]);
-  assert {:msg "  The network might not preserve the channel invariant"} R[Net#b] == (R[Net#d] + C[Net#d]);
-  assert {:msg "  The network might not preserve the channel invariant"} R[Net#d] == ((R[Net#b] + C[Net#b]) - 1);
-  assert {:msg "  The network might not preserve the channel invariant"} (forall idx$: int :: 
-    (0 <= idx$) && (idx$ < (R[Net#c] + C[Net#c])) ==> (M[Net#c][idx$] == (M[Net#a][idx$] + M[Net#b][idx$]))
+  R[Net#c] := R[Net#c] + (1 * Base#L);
+  I := R;
+  assert {:msg "  The network might not preserve the channel invariant (#44)"} (forall i: int :: 
+    (0 <= i) && (i < C[Net#a]) ==> (0 < M[Net#a][i])
   );
-  assert {:msg "  The network might not preserve the channel invariant"} (forall idx$: int :: 
-    (0 <= idx$) && (idx$ < (R[Net#d] + C[Net#d])) ==> (M[Net#d][idx$] == (M[Net#a][idx$] + M[Net#b][idx$]))
+  assert {:msg "  The network might not preserve the channel invariant (#45)"} R[Net#a] == C[Net#c];
+  assert {:msg "  The network might not preserve the channel invariant (#46)"} R[Net#b] == C[Net#c];
+  assert {:msg "  The network might not preserve the channel invariant (#47)"} R[Net#a] == C[Net#d];
+  assert {:msg "  The network might not preserve the channel invariant (#48)"} R[Net#b] == C[Net#d];
+  assert {:msg "  The network might not preserve the channel invariant (#49)"} R[Net#d] == (C[Net#b] - 1);
+  assert {:msg "  The network might not preserve the channel invariant (#50)"} (forall idx$: int :: 
+    (0 <= idx$) && (idx$ < C[Net#c]) ==> (M[Net#c][idx$] == (M[Net#a][idx$] + M[Net#b][idx$]))
   );
-  assert {:msg "  The network might not preserve the channel invariant"} (forall idx$: int :: 
-    (1 <= idx$) && (idx$ < (R[Net#b] + C[Net#b])) ==> (M[Net#b][idx$] == M[Net#d][idx$ - 1])
+  assert {:msg "  The network might not preserve the channel invariant (#51)"} (forall idx$: int :: 
+    (0 <= idx$) && (idx$ < C[Net#d]) ==> (M[Net#d][idx$] == (M[Net#a][idx$] + M[Net#b][idx$]))
   );
+  assert {:msg "  The network might not preserve the channel invariant (#52)"} (forall idx$: int :: 
+    (1 <= idx$) && (idx$ < C[Net#b]) ==> (M[Net#b][idx$] == M[Net#d][idx$ - 1])
+  );
+  assert {:msg "  22.15: The network might not preserve the channel invariant (#53)"} I[Net#a] == I[Net#c];
+  assert {:msg "  23.15: The network might not preserve the channel invariant (#54)"} M[Net#b][0] == 0;
   C[Net#b] := C[Net#b] - 1;
-  assert {:msg "  19.3: The network might leave unread tokens on channel a"} C[Net#a] == 0;
-  assert {:msg "  19.3: The network might leave unread tokens on channel b"} C[Net#b] == 0;
-  assert {:msg "  19.3: The network might not produce the specified number of tokens on output out"} C[Net#c] == 0;
-  assert {:msg "  19.3: The network might leave unread tokens on channel d"} C[Net#d] == 0;
+  assert {:msg "  14.3: The network might leave unread tokens on channel a"} (C[Net#a] - R[Net#a]) == 0;
+  assert {:msg "  14.3: The network might leave unread tokens on channel b"} (C[Net#b] - R[Net#b]) == 0;
+  assert {:msg "  14.3: The network might not produce the specified number of tokens on output out"} (C[Net#c] - R[Net#c]) == 0;
+  assert {:msg "  14.3: The network might leave unread tokens on channel d"} (C[Net#d] - R[Net#d]) == 0;
 }
